Added : induction principles

LRInduction.v
@@ -3,85 +3,103 @@ From MetaCoq.PCUIC Require Import PCUICAst PCUICAstUtils
   PCUICLiftSubst PCUICUnivSubst PCUICEquality PCUICUtils PCUICPosition.
 From MetaCoq.PCUIC Require Export PCUICCumulativitySpec.
 From MetaCoq.PCUIC Require Export PCUICCases PCUICNormal.
-Require Import MLTTTyping LogicalRelation Context.
+Require Import MLTTTyping LogicalRelation.
+
+Fixpoint LR_rec0
+  (c : context) (t : term) (rEq rTe : term -> Type)
+  (rTeEq  : term -> term -> Type) (lr : LR rec0 c t rEq rTe rTeEq ) : 
+  forall 
+  (P0 : forall {c t rEq rTe rTeEq} ,
+   @LR zero rec0 c t rEq rTe rTeEq  -> Type),
+  (forall (Γ : context) (A : term) (neA : [Γ ||-ne A]),
+    P0 (LRne rec0 neA))
+  ->
+  (forall (Γ : context) (A : term) (H0 : [ Γ ||-0Π A ]) (H1 : TyPiRel1 (LR rec0) H0),
+    (forall {Δ} (h : [ |- Δ]),
+      P0(H1.(_F1) h)) ->
+    (forall {Δ a} (h1 : [ |- Δ ]) 
+      (h2 : @Rel1Te _ rec0 Δ a (F H0) (_F H0 h1; H1.(_F1) h1)),
+      P0 (_G1 H1 h1 h2)) ->
+    P0 (LRPi rec0 H0 H1)) 
+  ->
+   P0 lr.
+Proof.   
+   intros.
+   destruct lr.
+   1,4 : inversion l_.
+   eapply X; try eassumption.
+   eapply X0; try eassumption;
+   destruct H1; destruct H0;
+   intros;
+   apply LR_rec0; try assumption.
+Defined.
+
+Check LR_rec0.
 
 (*TODO : get a good induction principle*)
 (*Scheme LR_rect := Induction for LR Sort Type.*)
-
-Definition TyRelToLR {l l' l_ Γ A} : 
-  [LogRelRec l l' l_ | Γ ||- A] -> [Γ ||-< l | A].
-  intro.
-  unfold TyUr.
-  destruct l.
-  inversion l_.
-  unfold LogRelRec in X.
-  cbn in *.
-  destruct X.
-  eapply (@LRPackMk Γ A _ relEq relTerm relEqTerm).
-  inversion relLR;
-  subst.
-  inversion l_0.
-  econstructor.
-  assert ([Γ ||-1Π A | LR (LogRelRec one)]).
-  destruct H.
-  econstructor; try eassumption.
-  eapply G_ext.
-  eapply (@LRPi one (LogRelRec one) Γ A).
-  inversion l_0.
-Admitted.
-
-Check recl one zero Oi.
-
-Definition test {Γ A}: [recl one zero Oi | Γ ||- A] -> True.
-  intro H.
-  cbn in H.
-  unfold Rel1Ty in H.
-  destruct H.
-Admitted.
-
-Print LR.
 Fixpoint LR_rec1 
-  (l : TypeLevel)  
   (c : context) (t : term) (rEq rTe : term -> Type)
-  (rTeEq  : term -> term -> Type) (lr : LR (recl l) c t rEq rTe rTeEq ) : 
+  (rTeEq  : term -> term -> Type) (lr : LR rec1 c t rEq rTe rTeEq ) : 
   forall 
-  (P : forall {l} (rec' : _) {c t rEq rTe rTeEq} ,
-   @LR l rec' c t rEq rTe rTeEq  -> Type),
-  (forall (Γ : context) (h : [  |- Γ]) (l' : TypeLevel)
-    (l_ : (l') << (l)),
-    P (recl l) (LRU (recl l) h l' l_)) 
+  (P0 : forall {c t rEq rTe rTeEq} ,
+   @LR zero rec0 c t rEq rTe rTeEq  -> Type)
+  (P1 : forall {c t rEq rTe rTeEq} ,
+   @LR one rec1 c t rEq rTe rTeEq  -> Type),
+  (forall (Γ : context) (A : term) (neA : [Γ ||-ne A]),
+    P0 (LRne rec0 neA)) 
+  ->
+  (forall (Γ : context) (A : term) (H0 : [ Γ ||-0Π A ]) (H1 : TyPiRel1 (LR rec0) H0),
+    (forall {Δ} (h : [ |- Δ]),
+      P0 (H1.(_F1) h)) ->
+    (forall {Δ a} (h1 : [ |- Δ ]) 
+      (h2 : @Rel1Te _ rec0 Δ a (F H0) (_F H0 h1; H1.(_F1) h1)),
+      P0 (_G1 H1 h1 h2)) ->
+    P0 (LRPi rec0 H0 H1)) 
+  ->
+
+
+  (forall (Γ : context) (h : [  |- Γ]) {l' l_},
+    P1 (LRU rec1 h l' l_)) 
   ->
   (forall (Γ : context) (A : term) (neA : [Γ ||-ne A]),
-    P (recl l) (LRne (recl l) neA)) 
+    P1 (LRne rec1 neA)) 
   ->
-  (forall (Γ : context) (A : term) (H : [Γ ||-1Π A | LR (recl l)]),
-    (forall {Δ} (h : [ |- Δ]),
-      P (recl l) (relLR (_F H h))) ->
-    (forall {Δ a} (h1 : [ |- Δ ]) 
-      (h2 : [ Δ  ||-0 a ::: (F H) | _F H h1 ]),
-      P (recl l) (relLR (_G H h1 h2))) ->
-    P (recl l) (LRPi (recl l) H)) 
+  (forall (Γ : context) (A : term) (H0 : [ Γ ||-0Π A ]) (H1 : TyPiRel1 (LR rec1) H0),
+  (forall {Δ} (h : [ |- Δ]),
+    P1 (H1.(_F1) h)) ->
+  (forall {Δ a} (h1 : [ |- Δ ]) 
+    (h2 : @Rel1Te _ rec1 Δ a (F H0) (_F H0 h1; H1.(_F1) h1)),
+    P1 (_G1 H1 h1 h2)) ->
+  P1 (LRPi rec1 H0 H1)) 
   ->
-  (forall (Γ : context) (A : term) (heq : l = one)
-    (H : [(recl one) zero Oi | Γ ||- A]),
-    
-    P _ H.(relLR) ->
-    P _ (LRemb _ Oi H)) ->
 
-  P _ lr.
+
+  (forall (Γ : context) (A : term) {l' l_}
+    (H : [kit0 | Γ ||- A]),
+    
+    P0 (projT2 H) ->
+    P1 (@LRemb _ _ _ _ l' l_ H)) ->
+
+    P1 lr.
 Proof.
   intros.
   destruct lr.
-  eapply X; try eassumption.
-  eapply X0; try eassumption.
-  2 : eapply X2; try eassumption.
-  destruct H.
-  eapply X1;
+  eapply X1; try eassumption.
+  eapply X2; try eassumption.
+  destruct H1;destruct H0.
+  eapply X3;
   intros;
-  apply LR_rec1; try assumption.
+  eapply LR_rec1; try eassumption.
+  eapply X4.
+  destruct H.
+  inversion l.
+  1, 4 : inversion l_0.
+  all : eapply LR_rec0; assumption.
 Defined.
 
-Polymorphic Definition LR_rect : forall 
+
+(*Definition LR_rect : forall 
   (l : TypeLevel)
   (rec : forall l' : TypeLevel, (l') << (l) -> LogRelKit)
   (P : forall {c : context} {t : term} {rEq rTe : term -> Type}
@@ -144,6 +162,4 @@ Polymorphic Definition LR_ind : forall
    (rTeEq  : term -> term -> Type) (lr : LR rec c t rEq rTe rTeEq ),
 
   P lr := LR_rect.
-  
-
-
+*)
